vera/VerilogToSMT.v
@@ -47,7 +47,7 @@ Equations cast_from_to (from to: N) (t : SMTLib.term) : SMTLib.term :=
   cast_from_to from to t with N.compare to from => {
     | Lt => SMTLib.Term_BVExtract (N.to_nat to - 1) 0 t
     (* smtlib concat is backwards *)
-    | Gt => SMTLib.Term_BVConcat t (SMTLib.Term_BVLit _ (BV.zeros (to - from)))
+    | Gt => SMTLib.Term_BVConcat (SMTLib.Term_BVLit _ (BV.zeros (to - from))) t
     | Eq => t
     }
 .
